Proved correctness of lamwf subst

Auto/Embedding/LCtx.lean
@@ -14,16 +14,6 @@ theorem pushLCtx.commFn (f : α → β) (lctx : Nat → α) (x : α) :
   (fun n => f (pushLCtx lctx x n)) = (fun n => pushLCtx (fun n => f (lctx n)) (f x) n) :=
   funext (pushLCtx.comm f lctx x)
 
-def pushLCtx.comm_cast₁ (f : α → β) (lctx : Nat → α) (g : β → Sort w) (x : α) :
-  (n : Nat) → (H : g (f (pushLCtx lctx x n))) → g (pushLCtx (fun n => f (lctx n)) (f x) n)
-| 0       => fun H => H
-| .succ _ => fun H => H
-
-def pushLCtx.comm_cast₂ (f : α → β) (lctx : Nat → α) (g : β → Sort w) (x : α) :
-  (n : Nat) → (H : g (pushLCtx (fun n => f (lctx n)) (f x) n)) → g (f (pushLCtx lctx x n))
-| 0       => fun H => H
-| .succ _ => fun H => H
-
 @[reducible] def pushLCtxDep {rty : Nat → α} {lctxty : α → Sort u}
   (lctx : ∀ n, lctxty (rty n)) {xty : α} (x : lctxty xty) : ∀ n, lctxty (pushLCtx rty xty n)
 | 0     => x
@@ -70,6 +60,11 @@ theorem pushLCtxAt.commFn (lctx : Nat → α) (f : α → β) (x : α) (pos : Na
   (fun n => f (pushLCtxAt lctx x pos n)) = (fun n => pushLCtxAt (fun n => f (lctx n)) (f x) pos n) :=
   funext (pushLCtxAt.comm f lctx x pos)
 
+-- Surprisingly, this is definitionally equal
+def pushLCtx_pushLCtxAt (lctx : Nat → α) (x y : α) (pos : Nat) :
+  pushLCtx (pushLCtxAt lctx x pos) y = pushLCtxAt (pushLCtx lctx y) x (Nat.succ pos)
+  := rfl
+
 def pushLCtxAtDep {rty : Nat → α} {lctxty : α → Sort u}
   (lctx : ∀ n, lctxty (rty n)) {xty : α} (x : lctxty xty) : (pos : Nat) → (n : Nat) → lctxty (pushLCtxAt rty xty pos n)
 | 0 => pushLCtxDep lctx x
@@ -105,9 +100,38 @@ theorem pushLCtxAtDep.absorb {rty : Nat → α} {lctxty : α → Sort u}
     (@pushLCtxAtDep _ rty lctxty lctx _ x pos) (@pushLCtxAtDep _ (lctxty ∘ rty) id lctx _ x pos) :=
   PSigmaEq.of_heq _ (HEq.funext _ _ (pushLCtxAtDep.absorbAux _ _ _)) (pushLCtxAt.commFn _ _ _ _)
 
+-- Surprisingly, this is definitionally equal
+def pushLCtxDep_pushLCtxAtDep {rty : Nat → α} {lctxty : α → Sort u}
+  (lctx : ∀ n, lctxty (rty n)) {xty : α} (x : lctxty xty) {yty : α} (y : lctxty yty) (pos : Nat) :
+  pushLCtxDep (pushLCtxAtDep lctx x pos) y = pushLCtxAtDep (pushLCtxDep lctx y) x (Nat.succ pos) := rfl
+
 def popLCtx (lctx : Nat → α) := fun n => lctx (n + 1)
 
-def popLCtxAt (lctx : Nat → α) (pos : Nat) :=
+def popLCtx.comm (f : α → β) (lctx : Nat → α) :
+  (n : Nat) → f (popLCtx lctx n) = popLCtx (f ∘ lctx) n := fun _ => rfl
+
+def popLCtx.commFn (f : α → β) (lctx : Nat → α) :
+  (fun n => f (popLCtx lctx n)) = (fun n => popLCtx (f ∘ lctx) n) := rfl
+
+def popLCtxDep {rty : Nat → α} {lctxty : α → Sort u}
+  (lctx : ∀ n, lctxty (rty n)) : ∀ n, lctxty (popLCtx rty n) :=
+  fun n => lctx (n + 1)
+
+def popLCtxDep.comm {α : Sort w} {β : α → Sort x} {rty : Nat → α} {lctxty : α → Sort u}
+  (f : ∀ (x : α), lctxty x → β x) (lctx : ∀ n, lctxty (rty n)) (n : Nat) :
+  f _ (popLCtxDep lctx n) = popLCtxDep (lctxty:=β) (fun n => f _ (lctx n)) n := rfl
+
+def popLCtxDep.absorbAux {rty : Nat → α} {lctxty : α → Sort u}
+  (lctx : ∀ n, lctxty (rty n)) (n : Nat) : HEq
+    (@popLCtxDep _ rty lctxty lctx n)
+    (@popLCtxDep _ (lctxty ∘ rty) id lctx n) := HEq.refl _
+
+theorem popLCtxDep.absorb {rty : Nat → α} {lctxty : α → Sort u} (lctx : ∀ n, lctxty (rty n)) :
+  PSigmaEq (fun (α : Nat → Sort u) => (∀ (n : Nat), α n))
+    (@popLCtxDep _ rty lctxty lctx) (@popLCtxDep _ (lctxty ∘ rty) id lctx) :=
+  PSigmaEq.of_heq _ (HEq.funext _ _ (popLCtxDep.absorbAux _)) (popLCtx.commFn _ _)
+
+def popLCtxAt (lctx : Nat → α) (pos : Nat) := 
   match pos with
   | 0 => popLCtx lctx
   | pos' + 1 => fun n =>
@@ -115,53 +139,74 @@ def popLCtxAt (lctx : Nat → α) (pos : Nat) :=
     | 0 => lctx 0
     | n' + 1 => popLCtxAt (fun n => lctx (Nat.succ n)) pos' n'
 
-def popLCtxAt.comm_cast₁ (lctx : Nat → α) (f : α → β) (g : β → Sort w) (pos : Nat) :
-  (n : Nat) → (H : g (f (popLCtxAt lctx pos n))) → g (popLCtxAt (fun n => f (lctx n)) pos n) :=
+def popLCtxAt.comm (lctx : Nat → α) (f : α → β) (pos : Nat) :
+  (n : Nat) → f (popLCtxAt lctx pos n) = popLCtxAt (f ∘ lctx) pos n :=
   match pos with
-  | 0 => fun _ H => H
+  | 0 => fun _ => rfl
   | pos' + 1 => fun n =>
     match n with
-    | 0 => fun H => H
-    | n' + 1 => fun H => popLCtxAt.comm_cast₁ _ _ _ pos' n' H
+    | 0 => rfl
+    | n' + 1 => popLCtxAt.comm (fun n => lctx (.succ n)) f pos' n'
 
-def popLCtxAt.comm_cast₂ (lctx : Nat → α) (f : α → β) (g : β → Sort w) (pos : Nat) :
-  (n : Nat) → (H : g (popLCtxAt (fun n => f (lctx n)) pos n)) → g (f (popLCtxAt lctx pos n)) :=
-  match pos with
-  | 0 => fun _ H => H
-  | pos' + 1 => fun n =>
-    match n with
-    | 0 => fun H => H
-    | n' + 1 => fun H => popLCtxAt.comm_cast₂ _ _ _ pos' n' H
+def popLCtxAt.commFn (lctx : Nat → α) (f : α → β) (pos : Nat) :
+  (fun n => f (popLCtxAt lctx pos n)) = (fun n => popLCtxAt (f ∘ lctx) pos n) :=
+  funext (popLCtxAt.comm lctx f pos)
 
-def popAt_pushAt_eq (lctx : Nat → α) (x : α) :
-  (pos : Nat) → (n : Nat) → popLCtxAt (pushLCtxAt lctx x pos) pos n = lctx n
+def popLCtxAtDep {rty : Nat → α} {lctxty : α → Sort u}
+  (lctx : ∀ n, lctxty (rty n)) : (pos : Nat) → (n : Nat) → lctxty (popLCtxAt rty pos n)
+| 0 => popLCtxDep lctx
+| pos' + 1 => fun n =>
+  match n with
+  | 0 => lctx 0
+  | n' + 1 => popLCtxAtDep (fun n => lctx (Nat.succ n)) pos' n'
+
+def popLCtxAtDep.absorbAux {rty : Nat → α} {lctxty : α → Sort u}
+  (lctx : ∀ n, lctxty (rty n)) : (pos : Nat) → (n : Nat) → HEq
+    (@popLCtxAtDep _ rty lctxty lctx pos n)
+    (@popLCtxAtDep _ (lctxty ∘ rty) id lctx pos n)
+| 0 => fun _ => HEq.refl _
+| pos' + 1 => fun n =>
+  match n with
+  | 0 => HEq.refl _
+  | n' + 1 => popLCtxAtDep.absorbAux (fun n => lctx (.succ n)) pos' n'
+
+def popLCtxAtDep.absorbAux' {rty : Nat → α} {lctxty : α → Sort u}
+  (lctx : ∀ n, lctxty (rty n)) (pos : Nat) (n : Nat) : HEq
+    (@popLCtxAtDep _ rty lctxty lctx pos n)
+    (@popLCtxAtDep _ id (lctxty ∘ rty) lctx pos n) :=
+  HEq.trans
+    (b := @popLCtxAtDep _ (lctxty ∘ rty) id lctx pos n)
+    (popLCtxAtDep.absorbAux lctx pos n)
+    (HEq.symm (@popLCtxAtDep.absorbAux _ id (lctxty ∘ rty) lctx pos n))
+
+def popLCtxAtDep.absorb {rty : Nat → α} {lctxty : α → Sort u} (lctx : ∀ n, lctxty (rty n)) (pos : Nat):
+  PSigmaEq (fun (α : Nat → Sort u) => (∀ (n : Nat), α n))
+    (@popLCtxAtDep _ rty lctxty lctx pos) (@popLCtxAtDep _ (lctxty ∘ rty) id lctx pos) :=
+  PSigmaEq.of_heq _ (HEq.funext _ _ (popLCtxAtDep.absorbAux _ _)) (popLCtxAt.commFn _ _ _)
+
+def popLCtxAtDep.comm {α : Sort w} {β : α → Sort x} {rty : Nat → α} {lctxty : α → Sort u}
+  (f : ∀ (x : α), lctxty x → β x) (lctx : ∀ n, lctxty (rty n)) :
+  (pos : Nat) → (n : Nat) → f _ (popLCtxAtDep lctx pos n) = popLCtxAtDep (lctxty:=β) (fun n => f _ (lctx n)) pos n
 | 0 => fun _ => rfl
 | pos' + 1 => fun n =>
   match n with
   | 0 => rfl
-  | n' + 1 => popAt_pushAt_eq (fun n => lctx (Nat.succ n)) x pos' n'
+  | n' + 1 => popLCtxAtDep.comm f (fun n => lctx (Nat.succ n)) pos' n'
 
-def popAt_pushAt_eqFn (lctx : Nat → α) (x : α) (pos : Nat) :
-  popLCtxAt (pushLCtxAt lctx x pos) pos = lctx :=
-  funext (fun n => popAt_pushAt_eq lctx x pos n)
-
+def popLCtxAt.commDep
+  {β : α → Sort u} (lctx : Nat → α) (f : ∀ (x : α), β x) :
+  (pos n : Nat) → f (popLCtxAt lctx pos n) = popLCtxAtDep (fun n => f (lctx n)) pos n
+| 0 => fun _ => rfl
+| pos' + 1 => fun n =>
+  match n with
+  | 0 => rfl
+  | n' + 1 => popLCtxAt.commDep (fun n => lctx (.succ n)) f pos' n'
+ 
 -- #reduce fun lctx => popLCtxAt lctx 3 4
 
 def popLCtxs (lctx : Nat → α) : (i : Nat) → Nat → α
 | 0 => lctx
 | i' + 1 => popLCtx (popLCtxs lctx i')
-
-def popLCtx.succ_cast₁ (lctx : Nat → α) (f : (Nat → α) → Sort u) (i : Nat)
-  (H : f (popLCtxs (popLCtx lctx) i)) : f (popLCtxs lctx (Nat.succ i)) :=
-  match i with
-  | 0 => H
-  | i' + 1 => popLCtx.succ_cast₁ lctx (fun lctx => f (popLCtx lctx)) i' H
-
-def popLCtx.succ_cast₂ (lctx : Nat → α) (f : (Nat → α) → Sort u) (i : Nat)
-  (H : f (popLCtxs lctx (Nat.succ i))) : f (popLCtxs (popLCtx lctx) i) :=
-  match i with
-  | 0 => H
-  | i' + 1 => popLCtx.succ_cast₂ lctx (fun lctx => f (popLCtx lctx)) i' H
 
 -- Definitional equality :
 -- #check fun lctx x => (Eq.refl _ : popLCtx (pushLCtx lctx x) = lctx)
@@ -178,5 +223,26 @@ def push_pop_eq (lctx : Nat → α) :
   pushLCtx (popLCtx lctx) (lctx 0) = lctx := by
   apply funext
   intro n; cases n <;> rfl
+
+def popAt_pushAt_eq (lctx : Nat → α) (x : α) :
+  (pos : Nat) → (n : Nat) → popLCtxAt (pushLCtxAt lctx x pos) pos n = lctx n
+| 0 => fun _ => rfl
+| pos' + 1 => fun n =>
+  match n with
+  | 0 => rfl
+  | n' + 1 => popAt_pushAt_eq (fun n => lctx (Nat.succ n)) x pos' n'
+
+def popAtDep_pushAtDep_eq
+  {α : Sort w} {rty : Nat → α} {lctxty : α → Sort u}
+  (lctx : ∀ n, lctxty (rty n)) {xty : α} (x : lctxty xty) : (pos n : Nat) →
+  HEq (@popLCtxAtDep _ (pushLCtxAt rty xty pos) lctxty
+        (@pushLCtxAtDep _ rty lctxty lctx xty x pos) pos n
+      )
+      (lctx n)
+| 0 => fun _ => HEq.rfl
+| pos' + 1 => fun n =>
+  match n with
+  | 0 => HEq.rfl
+  | n' + 1 => @popAtDep_pushAtDep_eq _ _ lctxty (fun n => lctx (Nat.succ n)) _ x pos' n'
 
 end Auto.Embedding
